Wrote up Debruijn Indices

03Debruijn/BigStep.thy
@@ -2,59 +2,59 @@ theory BigStep
   imports Termination
 begin
 
-inductive big_evald :: "dexpr \<Rightarrow> dexpr \<Rightarrow> bool" (infix "\<Down>\<^sub>d" 50) where
-  bevd_const [simp]: "DConst k \<Down>\<^sub>d DConst k"
-| bevd_lam [simp]: "DLam t e \<Down>\<^sub>d DLam t e"
-| bevd_app [simp]: "e\<^sub>1 \<Down>\<^sub>d DLam t e\<^sub>1' \<Longrightarrow> e\<^sub>2 \<Down>\<^sub>d v\<^sub>2 \<Longrightarrow> substd 0 v\<^sub>2 e\<^sub>1' \<Down>\<^sub>d v \<Longrightarrow> DApp e\<^sub>1 e\<^sub>2 \<Down>\<^sub>d v"
+inductive big_evald :: "expr\<^sub>d \<Rightarrow> expr\<^sub>d \<Rightarrow> bool" (infix "\<Down>\<^sub>d" 50) where
+  bevd_const [simp]: "Const\<^sub>d k \<Down>\<^sub>d Const\<^sub>d k"
+| bevd_lam [simp]: "Lam\<^sub>d t e \<Down>\<^sub>d Lam\<^sub>d t e"
+| bevd_app [simp]: "e\<^sub>1 \<Down>\<^sub>d Lam\<^sub>d t e\<^sub>1' \<Longrightarrow> e\<^sub>2 \<Down>\<^sub>d v\<^sub>2 \<Longrightarrow> subst\<^sub>d 0 v\<^sub>2 e\<^sub>1' \<Down>\<^sub>d v \<Longrightarrow> App\<^sub>d e\<^sub>1 e\<^sub>2 \<Down>\<^sub>d v"
 
-inductive_cases [elim]: "DVar x \<Down>\<^sub>d v"
-inductive_cases [elim]: "DConst k \<Down>\<^sub>d v"
-inductive_cases [elim]: "DLam t e \<Down>\<^sub>d v"
-inductive_cases [elim]: "DApp e\<^sub>1 e\<^sub>2 \<Down>\<^sub>d v"
+inductive_cases [elim]: "Var\<^sub>d x \<Down>\<^sub>d v"
+inductive_cases [elim]: "Const\<^sub>d k \<Down>\<^sub>d v"
+inductive_cases [elim]: "Lam\<^sub>d t e \<Down>\<^sub>d v"
+inductive_cases [elim]: "App\<^sub>d e\<^sub>1 e\<^sub>2 \<Down>\<^sub>d v"
 
-lemma [simp]: "e \<Down>\<^sub>d v \<Longrightarrow> vald v"
+lemma [simp]: "e \<Down>\<^sub>d v \<Longrightarrow> value\<^sub>d v"
   by (induction e v rule: big_evald.induct) simp_all
 
 theorem deterministimb: "e \<Down>\<^sub>d v \<Longrightarrow> e \<Down>\<^sub>d v' \<Longrightarrow> v = v'"
 proof (induction e v arbitrary: v' rule: big_evald.induct)
   case (bevd_const k)
-  thus ?case by (induction "DConst k" v' rule: big_evald.induct) simp_all
+  thus ?case by (induction "Const\<^sub>d k" v' rule: big_evald.induct) simp_all
 next
   case (bevd_lam t e)
-  thus ?case by (induction "DLam t e" v' rule: big_evald.induct) simp_all
+  thus ?case by (induction "Lam\<^sub>d t e" v' rule: big_evald.induct) simp_all
 next
   case (bevd_app e\<^sub>1 t e\<^sub>1' e\<^sub>2 v\<^sub>2 v)
   from bevd_app(7, 1, 2, 3, 4, 5, 6) show ?case 
-    by (induction "DApp e\<^sub>1 e\<^sub>2" v' rule: big_evald.induct) blast+
+    by (induction "App\<^sub>d e\<^sub>1 e\<^sub>2" v' rule: big_evald.induct) blast+
 qed
 
-lemma [simp]: "vald v \<Longrightarrow> v \<Down>\<^sub>d v"
+lemma [simp]: "value\<^sub>d v \<Longrightarrow> v \<Down>\<^sub>d v"
   by (induction v) simp_all
 
-lemma completeb' [simp]: "e \<leadsto>\<^sub>d e' \<Longrightarrow> e' \<Down>\<^sub>d v \<Longrightarrow> vald v \<Longrightarrow> e \<Down>\<^sub>d v"
-proof (induction e e' arbitrary: v rule: evald.induct)
-  case (evd_app3 e\<^sub>2 t e\<^sub>1)
+lemma completeb' [simp]: "e \<leadsto>\<^sub>d e' \<Longrightarrow> e' \<Down>\<^sub>d v \<Longrightarrow> value\<^sub>d v \<Longrightarrow> e \<Down>\<^sub>d v"
+proof (induction e e' arbitrary: v rule: eval\<^sub>d.induct)
+  case (ev\<^sub>d_app3 e\<^sub>2 t e\<^sub>1)
   moreover hence "e\<^sub>2 \<Down>\<^sub>d e\<^sub>2" by simp
   ultimately show ?case by (metis bevd_lam bevd_app)
 qed fastforce+
 
-theorem completeb [simp]: "iter (\<leadsto>\<^sub>d) e v \<Longrightarrow> vald v \<Longrightarrow> e \<Down>\<^sub>d v"
+theorem completeb [simp]: "iter (\<leadsto>\<^sub>d) e v \<Longrightarrow> value\<^sub>d v \<Longrightarrow> e \<Down>\<^sub>d v"
   by (induction e v rule: iter.induct) simp_all
 
-theorem progressb [simp]: "[] \<turnstile>\<^sub>d e : t \<Longrightarrow> \<exists>v. vald v \<and> e \<Down>\<^sub>d v"
+theorem progressb [simp]: "[] \<turnstile>\<^sub>d e : t \<Longrightarrow> \<exists>v. value\<^sub>d v \<and> e \<Down>\<^sub>d v"
 proof -
   assume "[] \<turnstile>\<^sub>d e : t"
-  then obtain v where "vald v \<and> iter (\<leadsto>\<^sub>d) e v" by fastforce
+  then obtain v where "value\<^sub>d v \<and> iter (\<leadsto>\<^sub>d) e v" by fastforce
   thus ?thesis by fastforce
 qed
 
 theorem correctb: "e \<Down>\<^sub>d v \<Longrightarrow> iter (\<leadsto>\<^sub>d) e v"
 proof (induction e v rule: big_evald.induct)
   case (bevd_app e\<^sub>1 t e\<^sub>1' e\<^sub>2 v\<^sub>2 v)
-  hence "iter (\<leadsto>\<^sub>d) (DApp e\<^sub>1 e\<^sub>2) (DApp (DLam t e\<^sub>1') e\<^sub>2)" by simp
-  moreover from bevd_app have "iter (\<leadsto>\<^sub>d) (DApp (DLam t e\<^sub>1') e\<^sub>2) (DApp (DLam t e\<^sub>1') v\<^sub>2)" by simp
-  moreover from bevd_app have "DApp (DLam t e\<^sub>1') v\<^sub>2 \<leadsto>\<^sub>d substd 0 v\<^sub>2 e\<^sub>1'" by simp
-  moreover from bevd_app have "iter (\<leadsto>\<^sub>d) (substd 0 v\<^sub>2 e\<^sub>1') v" by simp
+  hence "iter (\<leadsto>\<^sub>d) (App\<^sub>d e\<^sub>1 e\<^sub>2) (App\<^sub>d (Lam\<^sub>d t e\<^sub>1') e\<^sub>2)" by simp
+  moreover from bevd_app have "iter (\<leadsto>\<^sub>d) (App\<^sub>d (Lam\<^sub>d t e\<^sub>1') e\<^sub>2) (App\<^sub>d (Lam\<^sub>d t e\<^sub>1') v\<^sub>2)" by simp
+  moreover from bevd_app have "App\<^sub>d (Lam\<^sub>d t e\<^sub>1') v\<^sub>2 \<leadsto>\<^sub>d subst\<^sub>d 0 v\<^sub>2 e\<^sub>1'" by simp
+  moreover from bevd_app have "iter (\<leadsto>\<^sub>d) (subst\<^sub>d 0 v\<^sub>2 e\<^sub>1') v" by simp
   ultimately show ?case by (metis iter_append iter_step)
 qed simp_all
 
