03Debruijn/Multisubst.thy
@@ -1,16 +1,16 @@
 theory Multisubst
-  imports Debruijn
+  imports DebruijnIndices
 begin
 
-inductive tc_pairs :: "ty list \<Rightarrow> dexpr list \<Rightarrow> bool" where
+inductive tc_pairs :: "ty list \<Rightarrow> expr\<^sub>d list \<Rightarrow> bool" where
   tcp_nil [simp]: "tc_pairs [] []"
-| tcp_cons [simp]: "[] \<turnstile>\<^sub>d e : t \<Longrightarrow> vald e \<Longrightarrow> tc_pairs \<Gamma> es \<Longrightarrow> tc_pairs (t # \<Gamma>) (e # es)"
+| tcp_cons [simp]: "[] \<turnstile>\<^sub>d e : t \<Longrightarrow> value\<^sub>d e \<Longrightarrow> tc_pairs \<Gamma> es \<Longrightarrow> tc_pairs (t # \<Gamma>) (e # es)"
 
-primrec multisubst :: "dexpr list \<Rightarrow> dexpr \<Rightarrow> dexpr" where
+primrec multisubst :: "expr\<^sub>d list \<Rightarrow> expr\<^sub>d \<Rightarrow> expr\<^sub>d" where
   "multisubst [] e = e"
-| "multisubst (e' # es) e = multisubst es (substd 0 e' e)"
+| "multisubst (e' # es) e = multisubst es (subst\<^sub>d 0 e' e)"
 
-lemma [simp]: "tc_pairs \<Gamma> es \<Longrightarrow> vald e \<Longrightarrow> x \<le> length \<Gamma> \<Longrightarrow> [] \<turnstile>\<^sub>d e : t \<Longrightarrow> 
+lemma [simp]: "tc_pairs \<Gamma> es \<Longrightarrow> value\<^sub>d e \<Longrightarrow> x \<le> length \<Gamma> \<Longrightarrow> [] \<turnstile>\<^sub>d e : t \<Longrightarrow> 
   tc_pairs (insert_at x t \<Gamma>) (insert_at x e es)"
 proof (induction \<Gamma> es arbitrary: x rule: tc_pairs.induct)
   case (tcp_cons t' e' \<Gamma> es)
@@ -30,60 +30,43 @@ lemma [simp]: "[] \<turnstile>\<^sub>d e : t \<Longrightarrow> multisubst es e =
   by (induction es) simp_all
 
 lemma multisubst_var [simp]: "lookup vs x = Some v \<Longrightarrow> 
-    (\<And>v es. v \<in> set vs \<Longrightarrow> multisubst es v = v) \<Longrightarrow> multisubst vs (DVar x) = v"
+    (\<And>v es. v \<in> set vs \<Longrightarrow> multisubst es v = v) \<Longrightarrow> multisubst vs (Var\<^sub>d x) = v"
   by (induction vs x rule: lookup.induct) simp_all
 
-lemma [simp]: "multisubst es (DConst k) = DConst k"
+lemma [simp]: "multisubst es (Const\<^sub>d k) = Const\<^sub>d k"
   by (induction es) simp_all
 
-lemma [simp]: "\<exists>e'. multisubst es (DLam t e) = DLam t e'"
+lemma [simp]: "\<exists>e'. multisubst es (Lam\<^sub>d t e) = Lam\<^sub>d t e'"
   by (induction es arbitrary: e) simp_all
 
-lemma [simp]: "\<exists>e'. multisubst es (DLam t e) = DLam t e' \<and> 
-    (\<forall>e\<^sub>2. (\<forall>ee. substd 0 ee e\<^sub>2 = e\<^sub>2) \<longrightarrow> substd 0 e\<^sub>2 e' = multisubst es (substd 0 e\<^sub>2 e))"
+lemma [simp]: "\<exists>e'. multisubst es (Lam\<^sub>d t e) = Lam\<^sub>d t e' \<and> 
+    (\<forall>e\<^sub>2. (\<forall>ee. subst\<^sub>d 0 ee e\<^sub>2 = e\<^sub>2) \<longrightarrow> subst\<^sub>d 0 e\<^sub>2 e' = multisubst es (subst\<^sub>d 0 e\<^sub>2 e))"
   by (induction es arbitrary: e) simp_all
 
 lemma [simp]: "tc_pairs \<Gamma> es \<Longrightarrow> insert_at 0 t\<^sub>1 \<Gamma> \<turnstile>\<^sub>d e : t\<^sub>2 \<Longrightarrow> 
-  \<exists>e'. multisubst es (DLam t\<^sub>1 e) = DLam t\<^sub>1 e' \<and> ([t\<^sub>1] \<turnstile>\<^sub>d e' : t\<^sub>2) \<and>
-    (\<forall>e\<^sub>2. ([] \<turnstile>\<^sub>d e\<^sub>2 : t\<^sub>1) \<longrightarrow> multisubst (insert_at 0 e\<^sub>2 es) e = substd 0 e\<^sub>2 e')"
+  \<exists>e'. multisubst es (Lam\<^sub>d t\<^sub>1 e) = Lam\<^sub>d t\<^sub>1 e' \<and> ([t\<^sub>1] \<turnstile>\<^sub>d e' : t\<^sub>2) \<and>
+    (\<forall>e\<^sub>2. ([] \<turnstile>\<^sub>d e\<^sub>2 : t\<^sub>1) \<longrightarrow> multisubst (insert_at 0 e\<^sub>2 es) e = subst\<^sub>d 0 e\<^sub>2 e')"
 proof (induction \<Gamma> es arbitrary: e rule: tc_pairs.induct)
   case (tcp_cons e' t \<Gamma> es)
   hence "[] \<turnstile>\<^sub>d e' : t" by simp
   hence "\<Gamma> \<turnstile>\<^sub>d e' : t" using tc_postpend by fastforce
-  hence "insert_at 0 t\<^sub>1 \<Gamma> \<turnstile>\<^sub>d incrd 0 e' : t" by simp
-  with tcp_cons have "insert_at 0 t\<^sub>1 \<Gamma> \<turnstile>\<^sub>d substd (Suc 0) (incrd 0 e') e : t\<^sub>2" 
+  hence "insert_at 0 t\<^sub>1 \<Gamma> \<turnstile>\<^sub>d incr\<^sub>d 0 e' : t" by simp
+  with tcp_cons have "insert_at 0 t\<^sub>1 \<Gamma> \<turnstile>\<^sub>d subst\<^sub>d (Suc 0) (incr\<^sub>d 0 e') e : t\<^sub>2" 
     by (induction \<Gamma>) simp_all
   with tcp_cons obtain ee' where E: "([t\<^sub>1] \<turnstile>\<^sub>d ee' : t\<^sub>2) \<and> 
-    multisubst es (DLam t\<^sub>1 (substd (Suc 0) (incrd 0 e') e)) = DLam t\<^sub>1 ee' \<and> 
+    multisubst es (Lam\<^sub>d t\<^sub>1 (subst\<^sub>d (Suc 0) (incr\<^sub>d 0 e') e)) = Lam\<^sub>d t\<^sub>1 ee' \<and> 
       (\<forall>e\<^sub>2. ([] \<turnstile>\<^sub>d e\<^sub>2 : t\<^sub>1) \<longrightarrow> 
-        multisubst (insert_at 0 e\<^sub>2 es) (substd (Suc 0) (incrd 0 e') e) = substd 0 e\<^sub>2 ee')" 
+        multisubst (insert_at 0 e\<^sub>2 es) (subst\<^sub>d (Suc 0) (incr\<^sub>d 0 e') e) = subst\<^sub>d 0 e\<^sub>2 ee')" 
     by fastforce
   hence "\<And>e\<^sub>2. [] \<turnstile>\<^sub>d e\<^sub>2 : t\<^sub>1 \<Longrightarrow> 
-    multisubst es (substd 0 e\<^sub>2 (substd (Suc 0) (incrd 0 e') e)) = substd 0 e\<^sub>2 ee'" 
+    multisubst es (subst\<^sub>d 0 e\<^sub>2 (subst\<^sub>d (Suc 0) (incr\<^sub>d 0 e') e)) = subst\<^sub>d 0 e\<^sub>2 ee'" 
       by (induction es) simp_all
-  hence "\<And>e\<^sub>2. [] \<turnstile>\<^sub>d e\<^sub>2 : t\<^sub>1 \<Longrightarrow> multisubst es (substd 0 e' (substd 0 e\<^sub>2 e)) = substd 0 e\<^sub>2 ee'"
+  hence "\<And>e\<^sub>2. [] \<turnstile>\<^sub>d e\<^sub>2 : t\<^sub>1 \<Longrightarrow> multisubst es (subst\<^sub>d 0 e' (subst\<^sub>d 0 e\<^sub>2 e)) = subst\<^sub>d 0 e\<^sub>2 ee'"
     by fastforce
   with E show ?case by simp
 qed simp_all
 
-lemma [simp]: "multisubst es (DApp e\<^sub>1 e\<^sub>2) = DApp (multisubst es e\<^sub>1) (multisubst es e\<^sub>2)"
+lemma [simp]: "multisubst es (App\<^sub>d e\<^sub>1 e\<^sub>2) = App\<^sub>d (multisubst es e\<^sub>1) (multisubst es e\<^sub>2)"
   by (induction es arbitrary: e\<^sub>1 e\<^sub>2) simp_all
-
-lemma multisubst_val [simp]: "vald (multisubst es e) \<Longrightarrow> (\<And>e'. e' \<in> set es \<Longrightarrow> vald e') \<Longrightarrow> 
-  vald e \<or> (\<exists>x. e = DVar x \<and> x < length es)"
-proof (induction es arbitrary: e)
-  case (Cons e' es)
-  thus ?case
-  proof (cases "vald (substd 0 e' e)")
-    case True
-    with Cons have "vald e \<or> e = DVar 0" by simp
-    thus ?thesis by fastforce
-  next
-    case False
-    with Cons obtain x where "substd 0 e' e = DVar x \<and> x < length es" by fastforce
-    moreover with Cons have "e = DVar (Suc x)" by fastforce
-    ultimately show ?thesis by simp
-  qed
-qed simp_all
 
 end
