03Debruijn/Termination.thy
@@ -2,13 +2,13 @@ theory Termination
   imports Multisubst
 begin
 
-abbreviation terminatesd :: "dexpr \<Rightarrow> bool" where
-  "terminatesd e \<equiv> (\<exists>e'. vald e' \<and> iter (\<leadsto>\<^sub>d) e e')"
+abbreviation terminatesd :: "expr\<^sub>d \<Rightarrow> bool" where
+  "terminatesd e \<equiv> (\<exists>e'. value\<^sub>d e' \<and> iter (\<leadsto>\<^sub>d) e e')"
 
-primrec stable :: "ty \<Rightarrow> dexpr \<Rightarrow> bool" where
+primrec stable :: "ty \<Rightarrow> expr\<^sub>d \<Rightarrow> bool" where
   "stable Num e = (terminatesd e \<and> [] \<turnstile>\<^sub>d e : Num)"
 | "stable (Arrow t\<^sub>1 t\<^sub>2) e = (terminatesd e \<and> ([] \<turnstile>\<^sub>d e : Arrow t\<^sub>1 t\<^sub>2) \<and> 
-    (\<forall>e'. stable t\<^sub>1 e' \<longrightarrow> vald e' \<longrightarrow> stable t\<^sub>2 (DApp e e')))"
+    (\<forall>e'. stable t\<^sub>1 e' \<longrightarrow> value\<^sub>d e' \<longrightarrow> stable t\<^sub>2 (App\<^sub>d e e')))"
 
 lemma stable_typechecks: "stable t e \<Longrightarrow> [] \<turnstile>\<^sub>d e : t"
   by (induction t) simp_all
@@ -16,56 +16,59 @@ lemma stable_typechecks: "stable t e \<Longrightarrow> [] \<turnstile>\<^sub>d e
 lemma stable_terminates: "stable t e \<Longrightarrow> terminatesd e"
   by (induction t) simp_all
 
-lemma [simp]: "terminatesd (DConst k)"
+lemma [simp]: "terminatesd (Const\<^sub>d k)"
 proof
-  show "vald (DConst k) \<and> iter (\<leadsto>\<^sub>d) (DConst k) (DConst k)" by simp
+  show "value\<^sub>d (Const\<^sub>d k) \<and> iter (\<leadsto>\<^sub>d) (Const\<^sub>d k) (Const\<^sub>d k)" by simp
 qed
 
-lemma [simp]: "terminatesd (DLam t e)"
+lemma [simp]: "terminatesd (Lam\<^sub>d t e)"
 proof
-  show "vald (DLam t e) \<and> iter (\<leadsto>\<^sub>d) (DLam t e) (DLam t e)" by simp
+  show "value\<^sub>d (Lam\<^sub>d t e) \<and> iter (\<leadsto>\<^sub>d) (Lam\<^sub>d t e) (Lam\<^sub>d t e)" by simp
 qed
 
 lemma [simp]: "stable t e \<Longrightarrow> stable t (multisubst es e)"
 proof (induction es)
   case (Cons e' es)
   hence "[] \<turnstile>\<^sub>d e : t" by (metis stable_typechecks)
-  hence "substd 0 e' e = e" by simp
+  hence "subst\<^sub>d 0 e' e = e" by simp
   with Cons show ?case by simp
 qed simp_all
 
 lemma [simp]: "tc_pairs \<Gamma> es \<Longrightarrow> list_all2 stable \<Gamma> es \<Longrightarrow> lookup \<Gamma> x = Some t \<Longrightarrow> 
-  stable t (multisubst es (DVar x))"
+  stable t (multisubst es (Var\<^sub>d x))"
 proof (induction \<Gamma> es arbitrary: x rule: tc_pairs.induct)
   case (tcp_cons t' e \<Gamma> ves)
   thus ?case by (induction x) simp_all
 qed simp_all
 
+lemma evald_backwards: "iter (\<leadsto>\<^sub>d) e v \<Longrightarrow> value\<^sub>d v \<Longrightarrow> e \<leadsto>\<^sub>d e' \<Longrightarrow> iter (\<leadsto>\<^sub>d) e' v"
+  by (induction e v rule: iter.induct) (metis val_no_eval\<^sub>d, metis determinism\<^sub>d)
+
 lemma [simp]: "e \<leadsto>\<^sub>d e' \<Longrightarrow> terminatesd e = terminatesd e'"
 proof 
   assume "terminatesd e"
-  then obtain v where V: "vald v \<and> iter (\<leadsto>\<^sub>d) e v" by fastforce
+  then obtain v where V: "value\<^sub>d v \<and> iter (\<leadsto>\<^sub>d) e v" by fastforce
   moreover assume "e \<leadsto>\<^sub>d e'"
-  ultimately have "vald v \<and> iter (\<leadsto>\<^sub>d) e' v" by (metis evald_backwards)
+  ultimately have "value\<^sub>d v \<and> iter (\<leadsto>\<^sub>d) e' v" by (metis evald_backwards)
   thus "terminatesd e'" by fastforce
 next
   assume "terminatesd e'"
-  then obtain v where V: "vald v \<and> iter (\<leadsto>\<^sub>d) e' v" by fastforce
+  then obtain v where V: "value\<^sub>d v \<and> iter (\<leadsto>\<^sub>d) e' v" by fastforce
   moreover assume "e \<leadsto>\<^sub>d e'"
-  ultimately have "vald v \<and> iter (\<leadsto>\<^sub>d) e v" by (metis iter_step)
+  ultimately have "value\<^sub>d v \<and> iter (\<leadsto>\<^sub>d) e v" by (metis iter_step)
   thus "terminatesd e" by fastforce
 qed
 
 lemma stable_evald: "e \<leadsto>\<^sub>d e' \<Longrightarrow> stable t e \<Longrightarrow> stable t e'"
 proof (induction t arbitrary: e e')
   case (Arrow t\<^sub>1 t\<^sub>2)
-  moreover have "\<And>e\<^sub>2. stable t\<^sub>1 e\<^sub>2 \<Longrightarrow> vald e\<^sub>2 \<Longrightarrow> stable t\<^sub>2 (DApp e' e\<^sub>2)" 
+  moreover have "\<And>e\<^sub>2. stable t\<^sub>1 e\<^sub>2 \<Longrightarrow> value\<^sub>d e\<^sub>2 \<Longrightarrow> stable t\<^sub>2 (App\<^sub>d e' e\<^sub>2)" 
   proof -
     fix e\<^sub>2
-    assume "stable t\<^sub>1 e\<^sub>2" and "vald e\<^sub>2"
-    with Arrow have X: "stable t\<^sub>2 (DApp e e\<^sub>2)" by simp
-    from Arrow have "DApp e e\<^sub>2 \<leadsto>\<^sub>d DApp e' e\<^sub>2" by simp
-    with Arrow(2) X show "stable t\<^sub>2 (DApp e' e\<^sub>2)" by simp
+    assume "stable t\<^sub>1 e\<^sub>2" and "value\<^sub>d e\<^sub>2"
+    with Arrow have X: "stable t\<^sub>2 (App\<^sub>d e e\<^sub>2)" by simp
+    from Arrow have "App\<^sub>d e e\<^sub>2 \<leadsto>\<^sub>d App\<^sub>d e' e\<^sub>2" by simp
+    with Arrow(2) X show "stable t\<^sub>2 (App\<^sub>d e' e\<^sub>2)" by simp
   qed 
   ultimately show ?case by simp
 qed simp_all
@@ -78,15 +81,15 @@ proof (induction t arbitrary: e e')
   case (Arrow t\<^sub>1 t\<^sub>2)
   from Arrow have "terminatesd e'" by simp
   with Arrow have X: "terminatesd e" by fastforce
-  have "\<And>e\<^sub>2. stable t\<^sub>1 e\<^sub>2 \<Longrightarrow> vald e\<^sub>2 \<Longrightarrow> stable t\<^sub>2 (DApp e e\<^sub>2)" 
+  have "\<And>e\<^sub>2. stable t\<^sub>1 e\<^sub>2 \<Longrightarrow> value\<^sub>d e\<^sub>2 \<Longrightarrow> stable t\<^sub>2 (App\<^sub>d e e\<^sub>2)" 
   proof -
     fix e\<^sub>2
-    assume S: "stable t\<^sub>1 e\<^sub>2" and "vald e\<^sub>2"
-    with Arrow have Y: "stable t\<^sub>2 (DApp e' e\<^sub>2)" by simp
+    assume S: "stable t\<^sub>1 e\<^sub>2" and "value\<^sub>d e\<^sub>2"
+    with Arrow have Y: "stable t\<^sub>2 (App\<^sub>d e' e\<^sub>2)" by simp
     from S have "[] \<turnstile>\<^sub>d e\<^sub>2 : t\<^sub>1"  by (metis stable_typechecks)
-    with Arrow(3) have Z: "[] \<turnstile>\<^sub>d DApp e e\<^sub>2 : t\<^sub>2" by simp
-    from Arrow have "DApp e e\<^sub>2 \<leadsto>\<^sub>d DApp e' e\<^sub>2" by simp
-    with Arrow Y Z show "stable t\<^sub>2 (DApp e e\<^sub>2)" by blast
+    with Arrow(3) have Z: "[] \<turnstile>\<^sub>d App\<^sub>d e e\<^sub>2 : t\<^sub>2" by simp
+    from Arrow have "App\<^sub>d e e\<^sub>2 \<leadsto>\<^sub>d App\<^sub>d e' e\<^sub>2" by simp
+    with Arrow Y Z show "stable t\<^sub>2 (App\<^sub>d e e\<^sub>2)" by blast
   qed
   with Arrow X show ?case by simp
 qed simp_all
@@ -97,47 +100,64 @@ proof (induction e e' rule: iter.induct)
   thus ?case using stable_evald_back by fastforce
 qed simp_all
 
+lemma eval_under_app_fst [simp]: "iter (\<leadsto>\<^sub>d) e\<^sub>1 e\<^sub>1' \<Longrightarrow> iter (\<leadsto>\<^sub>d) (App\<^sub>d e\<^sub>1 e\<^sub>2) (App\<^sub>d e\<^sub>1' e\<^sub>2)"
+proof (induction e\<^sub>1 e\<^sub>1' rule: iter.induct)
+  case (iter_step e\<^sub>1 e\<^sub>1' e\<^sub>1'')
+  hence "App\<^sub>d e\<^sub>1 e\<^sub>2 \<leadsto>\<^sub>d App\<^sub>d e\<^sub>1' e\<^sub>2" by simp
+  moreover from iter_step have "iter (\<leadsto>\<^sub>d) (App\<^sub>d e\<^sub>1' e\<^sub>2) (App\<^sub>d e\<^sub>1'' e\<^sub>2)" by simp
+  ultimately show ?case by simp
+qed simp_all
+
+lemma eval_under_app_snd [simp]: "iter (\<leadsto>\<^sub>d) e\<^sub>2 e\<^sub>2' \<Longrightarrow> value\<^sub>d e\<^sub>1 \<Longrightarrow> 
+  iter (\<leadsto>\<^sub>d) (App\<^sub>d e\<^sub>1 e\<^sub>2) (App\<^sub>d e\<^sub>1 e\<^sub>2')"
+proof (induction e\<^sub>2 e\<^sub>2' rule: iter.induct)
+  case (iter_step e\<^sub>2 e\<^sub>2' e\<^sub>2'')
+  hence "App\<^sub>d e\<^sub>1 e\<^sub>2 \<leadsto>\<^sub>d App\<^sub>d e\<^sub>1 e\<^sub>2'" by simp
+  moreover from iter_step have "iter (\<leadsto>\<^sub>d) (App\<^sub>d e\<^sub>1 e\<^sub>2') (App\<^sub>d e\<^sub>1 e\<^sub>2'')" by simp
+  ultimately show ?case by simp
+qed simp_all
+
 lemma tc_stable [simp]: "\<Gamma> \<turnstile>\<^sub>d e : t \<Longrightarrow> tc_pairs \<Gamma> es \<Longrightarrow> list_all2 stable \<Gamma> es \<Longrightarrow> 
   stable t (multisubst es e)"
-proof (induction \<Gamma> e t arbitrary: es rule: typecheckd.induct)
-  case (tcd_lam t\<^sub>1 \<Gamma> e t\<^sub>2)
-  then obtain e' where E: "multisubst es (DLam t\<^sub>1 e) = DLam t\<^sub>1 e' \<and> ([t\<^sub>1] \<turnstile>\<^sub>d e' : t\<^sub>2) \<and> 
-    (\<forall>e\<^sub>2. ([] \<turnstile>\<^sub>d e\<^sub>2 : t\<^sub>1) \<longrightarrow> multisubst (insert_at 0 e\<^sub>2 es) e = substd 0 e\<^sub>2 e')" by fastforce
-  moreover have "\<And>e\<^sub>2. stable t\<^sub>1 e\<^sub>2 \<Longrightarrow> vald e\<^sub>2 \<Longrightarrow> stable t\<^sub>2 (DApp (DLam t\<^sub>1 e') e\<^sub>2)"
+proof (induction \<Gamma> e t arbitrary: es rule: typing\<^sub>d.induct)
+  case (tc\<^sub>d_lam t\<^sub>1 \<Gamma> e t\<^sub>2)
+  then obtain e' where E: "multisubst es (Lam\<^sub>d t\<^sub>1 e) = Lam\<^sub>d t\<^sub>1 e' \<and> ([t\<^sub>1] \<turnstile>\<^sub>d e' : t\<^sub>2) \<and> 
+    (\<forall>e\<^sub>2. ([] \<turnstile>\<^sub>d e\<^sub>2 : t\<^sub>1) \<longrightarrow> multisubst (insert_at 0 e\<^sub>2 es) e = subst\<^sub>d 0 e\<^sub>2 e')" by fastforce
+  moreover have "\<And>e\<^sub>2. stable t\<^sub>1 e\<^sub>2 \<Longrightarrow> value\<^sub>d e\<^sub>2 \<Longrightarrow> stable t\<^sub>2 (App\<^sub>d (Lam\<^sub>d t\<^sub>1 e') e\<^sub>2)"
   proof -
     fix e\<^sub>2
-    assume S: "stable t\<^sub>1 e\<^sub>2" and V: "vald e\<^sub>2"
+    assume S: "stable t\<^sub>1 e\<^sub>2" and V: "value\<^sub>d e\<^sub>2"
     hence E2: "[] \<turnstile>\<^sub>d e\<^sub>2 : t\<^sub>1" by (metis stable_typechecks)
     hence T: "\<exists>t. [] \<turnstile>\<^sub>d e\<^sub>2 : t" by fastforce
-    from tcd_lam S have "list_all2 stable (insert_at 0 t\<^sub>1 \<Gamma>) (insert_at 0 e\<^sub>2 es)" by simp
-    with tcd_lam have "tc_pairs (insert_at 0 t\<^sub>1 \<Gamma>) (insert_at 0 e\<^sub>2 es) \<Longrightarrow> 
+    from tc\<^sub>d_lam S have "list_all2 stable (insert_at 0 t\<^sub>1 \<Gamma>) (insert_at 0 e\<^sub>2 es)" by simp
+    with tc\<^sub>d_lam have "tc_pairs (insert_at 0 t\<^sub>1 \<Gamma>) (insert_at 0 e\<^sub>2 es) \<Longrightarrow> 
       stable t\<^sub>2 (multisubst (insert_at 0 e\<^sub>2 es) e)" by blast
-    with tcd_lam S V T E have "stable t\<^sub>2 (substd 0 e\<^sub>2 e')" by (simp add: stable_typechecks)
-    moreover with V have "DApp (DLam t\<^sub>1 e') e\<^sub>2 \<leadsto>\<^sub>d substd 0 e\<^sub>2 e'" by simp
-    moreover from E have "[] \<turnstile>\<^sub>d DLam t\<^sub>1 e' : Arrow t\<^sub>1 t\<^sub>2" by simp
-    moreover with E2 have "[] \<turnstile>\<^sub>d DApp (DLam t\<^sub>1 e') e\<^sub>2 : t\<^sub>2" by simp
-    ultimately show "stable t\<^sub>2 (DApp (DLam t\<^sub>1 e') e\<^sub>2)" by (metis stable_evald_back)
+    with tc\<^sub>d_lam S V T E have "stable t\<^sub>2 (subst\<^sub>d 0 e\<^sub>2 e')" by (simp add: stable_typechecks)
+    moreover with V have "App\<^sub>d (Lam\<^sub>d t\<^sub>1 e') e\<^sub>2 \<leadsto>\<^sub>d subst\<^sub>d 0 e\<^sub>2 e'" by simp
+    moreover from E have "[] \<turnstile>\<^sub>d Lam\<^sub>d t\<^sub>1 e' : Arrow t\<^sub>1 t\<^sub>2" by simp
+    moreover with E2 have "[] \<turnstile>\<^sub>d App\<^sub>d (Lam\<^sub>d t\<^sub>1 e') e\<^sub>2 : t\<^sub>2" by simp
+    ultimately show "stable t\<^sub>2 (App\<^sub>d (Lam\<^sub>d t\<^sub>1 e') e\<^sub>2)" by (metis stable_evald_back)
   qed
   ultimately show ?case by simp
 next
-  case (tcd_app \<Gamma> e\<^sub>1 t\<^sub>1 t\<^sub>2 e\<^sub>2)
+  case (tc\<^sub>d_app \<Gamma> e\<^sub>1 t\<^sub>1 t\<^sub>2 e\<^sub>2)
   hence "terminatesd (multisubst es e\<^sub>2)" by (metis stable_terminates)
-  then obtain v\<^sub>2 where V2: "vald v\<^sub>2 \<and> iter (\<leadsto>\<^sub>d) (multisubst es e\<^sub>2) v\<^sub>2" by fastforce
-  with tcd_app have V2S: "stable t\<^sub>1 v\<^sub>2" by (metis stable_persists)
-  from tcd_app have "terminatesd (multisubst es e\<^sub>1)" by fastforce
-  then obtain v\<^sub>1 where V1: "vald v\<^sub>1 \<and> iter (\<leadsto>\<^sub>d) (multisubst es e\<^sub>1) v\<^sub>1" by fastforce
-  with tcd_app have SV: "stable (Arrow t\<^sub>1 t\<^sub>2) v\<^sub>1" by (metis stable_persists)
-  with V2S V2 have "stable t\<^sub>2 (DApp v\<^sub>1 v\<^sub>2)" by simp
-  moreover from V1 V2 have "iter (\<leadsto>\<^sub>d) (DApp v\<^sub>1 (multisubst es e\<^sub>2)) (DApp v\<^sub>1 v\<^sub>2)" by simp
+  then obtain v\<^sub>2 where V2: "value\<^sub>d v\<^sub>2 \<and> iter (\<leadsto>\<^sub>d) (multisubst es e\<^sub>2) v\<^sub>2" by fastforce
+  with tc\<^sub>d_app have V2S: "stable t\<^sub>1 v\<^sub>2" by (metis stable_persists)
+  from tc\<^sub>d_app have "terminatesd (multisubst es e\<^sub>1)" by fastforce
+  then obtain v\<^sub>1 where V1: "value\<^sub>d v\<^sub>1 \<and> iter (\<leadsto>\<^sub>d) (multisubst es e\<^sub>1) v\<^sub>1" by fastforce
+  with tc\<^sub>d_app have SV: "stable (Arrow t\<^sub>1 t\<^sub>2) v\<^sub>1" by (metis stable_persists)
+  with V2S V2 have "stable t\<^sub>2 (App\<^sub>d v\<^sub>1 v\<^sub>2)" by simp
+  moreover from V1 V2 have "iter (\<leadsto>\<^sub>d) (App\<^sub>d v\<^sub>1 (multisubst es e\<^sub>2)) (App\<^sub>d v\<^sub>1 v\<^sub>2)" by simp
   moreover from SV have "[] \<turnstile>\<^sub>d v\<^sub>1 : Arrow t\<^sub>1 t\<^sub>2" by simp
-  moreover with tcd_app have "[] \<turnstile>\<^sub>d DApp v\<^sub>1 (multisubst es e\<^sub>2) : t\<^sub>2" by simp
-  ultimately have X: "stable t\<^sub>2 (DApp v\<^sub>1 (multisubst es e\<^sub>2))" by (metis stable_persists_back)
-  from V1 have Y: "iter (\<leadsto>\<^sub>d) (DApp (multisubst es e\<^sub>1) (multisubst es e\<^sub>2)) 
-    (DApp v\<^sub>1 (multisubst es e\<^sub>2))" by simp
-  from tcd_app have "[] \<turnstile>\<^sub>d multisubst es e\<^sub>1 : Arrow t\<^sub>1 t\<^sub>2" by simp
-  moreover from tcd_app have "[] \<turnstile>\<^sub>d multisubst es e\<^sub>2 : t\<^sub>1" by simp
-  ultimately have "[] \<turnstile>\<^sub>d DApp (multisubst es e\<^sub>1) (multisubst es e\<^sub>2) : t\<^sub>2" by simp
-  with X Y have "stable t\<^sub>2 (DApp (multisubst es e\<^sub>1) (multisubst es e\<^sub>2))" 
+  moreover with tc\<^sub>d_app have "[] \<turnstile>\<^sub>d App\<^sub>d v\<^sub>1 (multisubst es e\<^sub>2) : t\<^sub>2" by simp
+  ultimately have X: "stable t\<^sub>2 (App\<^sub>d v\<^sub>1 (multisubst es e\<^sub>2))" by (metis stable_persists_back)
+  from V1 have Y: "iter (\<leadsto>\<^sub>d) (App\<^sub>d (multisubst es e\<^sub>1) (multisubst es e\<^sub>2)) 
+    (App\<^sub>d v\<^sub>1 (multisubst es e\<^sub>2))" by simp
+  from tc\<^sub>d_app have "[] \<turnstile>\<^sub>d multisubst es e\<^sub>1 : Arrow t\<^sub>1 t\<^sub>2" by simp
+  moreover from tc\<^sub>d_app have "[] \<turnstile>\<^sub>d multisubst es e\<^sub>2 : t\<^sub>1" by simp
+  ultimately have "[] \<turnstile>\<^sub>d App\<^sub>d (multisubst es e\<^sub>1) (multisubst es e\<^sub>2) : t\<^sub>2" by simp
+  with X Y have "stable t\<^sub>2 (App\<^sub>d (multisubst es e\<^sub>1) (multisubst es e\<^sub>2))" 
     by (metis stable_persists_back)
   thus ?case by simp
 qed simp_all
