04Stack/Stack.thy
@@ -1,18 +1,18 @@
 theory Stack
-  imports "../03Debruijn/Debruijn"
+  imports "../03Debruijn/DebruijnIndices"
 begin
 
 datatype frame = 
-  FApp1 dexpr
-  | FApp2 dexpr
+  FApp1 expr\<^sub>d
+  | FApp2 expr\<^sub>d
   | FReturn
 
-datatype stack_state = SS bool "frame list" dexpr
+datatype stack_state = SS bool "frame list" expr\<^sub>d
 
 inductive typecheck_stack :: "frame list \<Rightarrow> ty \<Rightarrow> ty \<Rightarrow> bool" (infix ": _ \<rightarrow>" 50) where
   tcs_nil [simp]: "[] : t \<rightarrow> t"
 | tcs_cons_app1 [simp]: "[] \<turnstile>\<^sub>d e : t\<^sub>1 \<Longrightarrow> s : t\<^sub>2 \<rightarrow> t \<Longrightarrow> FApp1 e # s : Arrow t\<^sub>1 t\<^sub>2 \<rightarrow> t"
-| tcs_cons_app2 [simp]: "[] \<turnstile>\<^sub>d e : Arrow t\<^sub>1 t\<^sub>2 \<Longrightarrow> vald e \<Longrightarrow> s : t\<^sub>2 \<rightarrow> t \<Longrightarrow> FApp2 e # s : t\<^sub>1 \<rightarrow> t"
+| tcs_cons_app2 [simp]: "[] \<turnstile>\<^sub>d e : Arrow t\<^sub>1 t\<^sub>2 \<Longrightarrow> value\<^sub>d e \<Longrightarrow> s : t\<^sub>2 \<rightarrow> t \<Longrightarrow> FApp2 e # s : t\<^sub>1 \<rightarrow> t"
 | tcs_cons_ret [simp]: "s : t' \<rightarrow> t \<Longrightarrow> FReturn # s : t' \<rightarrow> t"
 
 inductive_cases [elim]: "[] : t' \<rightarrow> t"
@@ -21,43 +21,43 @@ inductive_cases [elim]: "FApp2 e # s : t' \<rightarrow> t"
 inductive_cases [elim]: "FReturn # s : t' \<rightarrow> t"
 
 inductive typecheck_stack_state :: "stack_state \<Rightarrow> ty \<Rightarrow> bool" (infix ":\<^sub>s" 50) where
-  tcs_state [simp]: "s : t' \<rightarrow> t \<Longrightarrow> [] \<turnstile>\<^sub>d e : t' \<Longrightarrow> (b \<Longrightarrow> vald e) \<Longrightarrow> SS b s e :\<^sub>s t"
+  tcs_state [simp]: "s : t' \<rightarrow> t \<Longrightarrow> [] \<turnstile>\<^sub>d e : t' \<Longrightarrow> (b \<Longrightarrow> value\<^sub>d e) \<Longrightarrow> SS b s e :\<^sub>s t"
 
 inductive_cases [elim]: "SS b s e :\<^sub>s t"
 
 inductive evals :: "stack_state \<Rightarrow> stack_state \<Rightarrow> bool" (infix "\<leadsto>\<^sub>s" 50) where
-  evs_const [simp]: "SS False s (DConst k) \<leadsto>\<^sub>s SS True s (DConst k)"
-| evs_lam [simp]: "SS False s (DLam t e) \<leadsto>\<^sub>s SS True s (DLam t e)"
-| evs_app1 [simp]: "SS False s (DApp e\<^sub>1 e\<^sub>2) \<leadsto>\<^sub>s SS False (FApp1 e\<^sub>2 # s) e\<^sub>1"
+  evs_const [simp]: "SS False s (Const\<^sub>d k) \<leadsto>\<^sub>s SS True s (Const\<^sub>d k)"
+| evs_lam [simp]: "SS False s (Lam\<^sub>d t e) \<leadsto>\<^sub>s SS True s (Lam\<^sub>d t e)"
+| evs_app1 [simp]: "SS False s (App\<^sub>d e\<^sub>1 e\<^sub>2) \<leadsto>\<^sub>s SS False (FApp1 e\<^sub>2 # s) e\<^sub>1"
 | evs_app2 [simp]: "SS True (FApp1 e\<^sub>2 # s) e\<^sub>1 \<leadsto>\<^sub>s SS False (FApp2 e\<^sub>1 # s) e\<^sub>2"
-| evs_app3 [simp]: "SS True (FApp2 (DLam t e\<^sub>1) # s) e\<^sub>2 \<leadsto>\<^sub>s SS False (FReturn # s) (substd 0 e\<^sub>2 e\<^sub>1)"
+| evs_app3 [simp]: "SS True (FApp2 (Lam\<^sub>d t e\<^sub>1) # s) e\<^sub>2 \<leadsto>\<^sub>s SS False (FReturn # s) (subst\<^sub>d 0 e\<^sub>2 e\<^sub>1)"
 | evs_ret [simp]: "SS True (FReturn # s) e \<leadsto>\<^sub>s SS True s e"
 
 lemma [simp]: "[] \<turnstile>\<^sub>d e : t \<Longrightarrow> \<exists>\<Sigma>'. SS False s e \<leadsto>\<^sub>s \<Sigma>'"
-proof (induction "[] :: ty list" e t rule: typecheckd.induct)
-  case (tcd_const k)
-  have "SS False s (DConst k) \<leadsto>\<^sub>s SS True s (DConst k)" by simp
+proof (induction "[] :: ty list" e t rule: typing\<^sub>d.induct)
+  case (tc\<^sub>d_const k)
+  have "SS False s (Const\<^sub>d k) \<leadsto>\<^sub>s SS True s (Const\<^sub>d k)" by simp
   thus ?case by fastforce
 next
-  case (tcd_lam t\<^sub>1 e t\<^sub>2)
-  have "SS False s (DLam t\<^sub>1 e) \<leadsto>\<^sub>s SS True s (DLam t\<^sub>1 e)" by simp
+  case (tc\<^sub>d_lam t\<^sub>1 e t\<^sub>2)
+  have "SS False s (Lam\<^sub>d t\<^sub>1 e) \<leadsto>\<^sub>s SS True s (Lam\<^sub>d t\<^sub>1 e)" by simp
   thus ?case by fastforce
 next
-  case (tcd_app e\<^sub>1 t\<^sub>1 t\<^sub>2 e\<^sub>2)
-  have "SS False s (DApp e\<^sub>1 e\<^sub>2) \<leadsto>\<^sub>s SS False (FApp1 e\<^sub>2 # s) e\<^sub>1" by simp
+  case (tc\<^sub>d_app e\<^sub>1 t\<^sub>1 t\<^sub>2 e\<^sub>2)
+  have "SS False s (App\<^sub>d e\<^sub>1 e\<^sub>2) \<leadsto>\<^sub>s SS False (FApp1 e\<^sub>2 # s) e\<^sub>1" by simp
   thus ?case by fastforce
 qed simp_all
 
-lemma [simp]: "s : t' \<rightarrow> t \<Longrightarrow> [] \<turnstile>\<^sub>d e : t' \<Longrightarrow> vald e \<Longrightarrow> s = [] \<or> (\<exists>\<Sigma>'. SS True s e \<leadsto>\<^sub>s \<Sigma>')"
+lemma [simp]: "s : t' \<rightarrow> t \<Longrightarrow> [] \<turnstile>\<^sub>d e : t' \<Longrightarrow> value\<^sub>d e \<Longrightarrow> s = [] \<or> (\<exists>\<Sigma>'. SS True s e \<leadsto>\<^sub>s \<Sigma>')"
 proof (induction s t' t rule: typecheck_stack.induct)
   case (tcs_cons_app1 e\<^sub>2 t\<^sub>1 s t\<^sub>2 t)
   hence "SS True (FApp1 e\<^sub>2 # s) e \<leadsto>\<^sub>s SS False (FApp2 e # s) e\<^sub>2" by simp
   thus ?case by fastforce
 next
   case (tcs_cons_app2 e\<^sub>1 t\<^sub>1 t\<^sub>2 s t)
-  then obtain e\<^sub>1' where "e\<^sub>1 = DLam t\<^sub>1 e\<^sub>1' \<and> insert_at 0 t\<^sub>1 [] \<turnstile>\<^sub>d e\<^sub>1' : t\<^sub>2" by blast
-  moreover with tcs_cons_app2 have "SS True (FApp2 (DLam t\<^sub>1 e\<^sub>1') # s) e \<leadsto>\<^sub>s 
-    SS False (FReturn # s) (substd 0 e e\<^sub>1')" by simp
+  then obtain e\<^sub>1' where "e\<^sub>1 = Lam\<^sub>d t\<^sub>1 e\<^sub>1' \<and> insert_at 0 t\<^sub>1 [] \<turnstile>\<^sub>d e\<^sub>1' : t\<^sub>2" by blast
+  moreover with tcs_cons_app2 have "SS True (FApp2 (Lam\<^sub>d t\<^sub>1 e\<^sub>1') # s) e \<leadsto>\<^sub>s 
+    SS False (FReturn # s) (subst\<^sub>d 0 e e\<^sub>1')" by simp
   ultimately show ?case by fastforce
 next 
   case (tcs_cons_ret s t')
@@ -65,7 +65,7 @@ next
   thus ?case by fastforce
 qed simp_all
 
-theorem progresss: "\<Sigma> :\<^sub>s t \<Longrightarrow> (\<exists>e. \<Sigma> = SS True [] e \<and> vald e) \<or> (\<exists>\<Sigma>'. \<Sigma> \<leadsto>\<^sub>s \<Sigma>')"
+theorem progresss: "\<Sigma> :\<^sub>s t \<Longrightarrow> (\<exists>e. \<Sigma> = SS True [] e \<and> value\<^sub>d e) \<or> (\<exists>\<Sigma>'. \<Sigma> \<leadsto>\<^sub>s \<Sigma>')"
 proof (induction \<Sigma> t rule: typecheck_stack_state.induct)
   case (tcs_state s t' t e b)
   thus ?case by (cases b) simp_all
@@ -80,13 +80,13 @@ proof (induction \<Sigma> \<Sigma>' rule: evals.induct)
 next
   case (evs_app2 e\<^sub>2 s e\<^sub>1)
   then obtain t\<^sub>1 t\<^sub>2 where X: "[] \<turnstile>\<^sub>d e\<^sub>2 : t\<^sub>1" and "s : t\<^sub>2 \<rightarrow> t" and "[] \<turnstile>\<^sub>d e\<^sub>1 : Arrow t\<^sub>1 t\<^sub>2" 
-   and "vald e\<^sub>1" by blast
+   and "value\<^sub>d e\<^sub>1" by blast
   with evs_app2 have "FApp2 e\<^sub>1 # s : t\<^sub>1 \<rightarrow> t" by simp
   with X show ?case by simp
 next
   case (evs_app3 t\<^sub>1 e\<^sub>1 s e\<^sub>2)
   then obtain t\<^sub>2 where "[t\<^sub>1] \<turnstile>\<^sub>d e\<^sub>1 : t\<^sub>2" and X: "s : t\<^sub>2 \<rightarrow> t" and "[] \<turnstile>\<^sub>d e\<^sub>2 : t\<^sub>1" by fastforce
-  hence "[] \<turnstile>\<^sub>d substd 0 e\<^sub>2 e\<^sub>1 : t\<^sub>2" by simp
+  hence "[] \<turnstile>\<^sub>d subst\<^sub>d 0 e\<^sub>2 e\<^sub>1 : t\<^sub>2" by simp
   moreover from X have "FReturn # s : t\<^sub>2 \<rightarrow> t" by simp
   ultimately show ?case by simp
 qed fastforce+
@@ -97,19 +97,19 @@ lemma [simp]: "iter (\<leadsto>\<^sub>s) \<Sigma> \<Sigma>' \<Longrightarrow> \<
 theorem determinisms: "\<Sigma> \<leadsto>\<^sub>s \<Sigma>' \<Longrightarrow> \<Sigma> \<leadsto>\<^sub>s \<Sigma>'' \<Longrightarrow> \<Sigma> :\<^sub>s t \<Longrightarrow> \<Sigma>' = \<Sigma>''"
 proof (induction \<Sigma> \<Sigma>' rule: evals.induct)
   case (evs_const s k)
-  thus ?case by (induction "SS False s (DConst k)" \<Sigma>'' rule: evals.induct) simp_all
+  thus ?case by (induction "SS False s (Const\<^sub>d k)" \<Sigma>'' rule: evals.induct) simp_all
 next
   case (evs_lam s t e)
-  thus ?case by (induction "SS False s (DLam t e)" \<Sigma>'' rule: evals.induct) simp_all
+  thus ?case by (induction "SS False s (Lam\<^sub>d t e)" \<Sigma>'' rule: evals.induct) simp_all
 next
   case (evs_app1 s e\<^sub>1 e\<^sub>2)
-  thus ?case by (induction "SS False s (DApp e\<^sub>1 e\<^sub>2)" \<Sigma>'' rule: evals.induct) simp_all
+  thus ?case by (induction "SS False s (App\<^sub>d e\<^sub>1 e\<^sub>2)" \<Sigma>'' rule: evals.induct) simp_all
 next
   case (evs_app2 e\<^sub>2 s e\<^sub>1)
   thus ?case by (induction "SS True (FApp1 e\<^sub>2 # s) e\<^sub>1" \<Sigma>'' rule: evals.induct) simp_all
 next
   case (evs_app3 t e\<^sub>1 s e\<^sub>2)
-  thus ?case by (induction "SS True (FApp2 (DLam t e\<^sub>1) # s) e\<^sub>2" \<Sigma>'' rule: evals.induct) simp_all
+  thus ?case by (induction "SS True (FApp2 (Lam\<^sub>d t e\<^sub>1) # s) e\<^sub>2" \<Sigma>'' rule: evals.induct) simp_all
 next 
   case (evs_ret s e)
   thus ?case by (induction "SS True (FReturn # s) e" \<Sigma>'' rule: evals.induct) simp_all
@@ -137,28 +137,28 @@ proof (induction s arbitrary: t')
   thus ?case 
   proof (induction f)
     case (FApp2 e)
-    then obtain t\<^sub>2 where X: "([] \<turnstile>\<^sub>d e : Arrow t' t\<^sub>2) \<and> vald e \<and> (s @ s' : t\<^sub>2 \<rightarrow> t)" by auto
+    then obtain t\<^sub>2 where X: "([] \<turnstile>\<^sub>d e : Arrow t' t\<^sub>2) \<and> value\<^sub>d e \<and> (s @ s' : t\<^sub>2 \<rightarrow> t)" by auto
     with FApp2 obtain t'' where "(s : t\<^sub>2 \<rightarrow> t'') \<and> (s' : t'' \<rightarrow> t)" by blast
     moreover with X have "FApp2 e # s : t' \<rightarrow> t''" by fastforce
     ultimately show ?case by blast
   qed force+
 qed force+
 
-lemma [simp]: "vald e \<Longrightarrow> iter (\<leadsto>\<^sub>s) (SS b s e) (SS True s e)"
+lemma [simp]: "value\<^sub>d e \<Longrightarrow> iter (\<leadsto>\<^sub>s) (SS b s e) (SS True s e)"
 proof (induction e)
-  case (DConst x)
+  case (Const\<^sub>d x)
   thus ?case 
   proof (induction b)
     case False
-    have "SS False s (DConst x) \<leadsto>\<^sub>s SS True s (DConst x)" by simp
+    have "SS False s (Const\<^sub>d x) \<leadsto>\<^sub>s SS True s (Const\<^sub>d x)" by simp
     thus ?case by (metis iter_step iter_refl)
   qed simp_all
 next
-  case (DLam t e)
+  case (Lam\<^sub>d t e)
   thus ?case
   proof (induction b)
     case False
-    have "SS False s (DLam t e) \<leadsto>\<^sub>s SS True s (DLam t e)" by simp
+    have "SS False s (Lam\<^sub>d t e) \<leadsto>\<^sub>s SS True s (Lam\<^sub>d t e)" by simp
     thus ?case by (metis iter_step iter_refl)
   qed simp_all
 qed simp_all
