03Debruijn/DebruijnIndices.thy
@@ -1,0 +1,201 @@
+theory DebruijnIndices
+  imports "../02Typed/Type" "../00Utils/Environment" "../00Utils/Iteration"
+begin
+
+section \<open>Debruijn Indices\<close>
+
+text \<open>Our next stage is the Debruijn-indexed language. It resembles the typed source language, but
+without names on the binders and with natural numbers for variables; these are our indices. Pierce 
+[5] covers Debruijn indices well, but the brief version is that it is a nameless representation of 
+expressions where a variable points to its binder by counting how many binders lie between them. So,
+for example, \<open>\<lambda>x. \<lambda>y. x y (\<lambda>y. x y)\<close> would be represented by \<open>\<lambda>. \<lambda>. 1 0 (\<lambda>. 2 0)\<close>. It is far more
+difficult to read, but has the great virtue that name-shadowing and name-collisions are impossible - 
+since there are no names - and thus substitution is made much simpler.\<close>
+
+datatype expr\<^sub>d = 
+  Var\<^sub>d nat
+  | Const\<^sub>d nat
+  | Lam\<^sub>d ty expr\<^sub>d
+  | App\<^sub>d expr\<^sub>d expr\<^sub>d
+
+text \<open>The typing relation remains similar to the source language typing relation, but notice that 
+the context is now a \<open>ty list\<close> examined with \<open>lookup\<close> rather than a \<open>var \<rightharpoonup> ty\<close> partial function, 
+and that binding a new variable is just consing to the front of the list - this automatically 
+increments all the other in-scope variables.\<close>
+
+inductive typing\<^sub>d :: "ty list \<Rightarrow> expr\<^sub>d \<Rightarrow> ty \<Rightarrow> bool" (infix "\<turnstile>\<^sub>d _ :" 50) where
+  tc\<^sub>d_var [simp]: "lookup \<Gamma> x = Some t \<Longrightarrow> \<Gamma> \<turnstile>\<^sub>d Var\<^sub>d x : t"
+| tc\<^sub>d_const [simp]: "\<Gamma> \<turnstile>\<^sub>d Const\<^sub>d n : Num"
+| tc\<^sub>d_lam [simp]: "insert_at 0 t\<^sub>1 \<Gamma> \<turnstile>\<^sub>d e : t\<^sub>2 \<Longrightarrow> \<Gamma> \<turnstile>\<^sub>d Lam\<^sub>d t\<^sub>1 e : Arrow t\<^sub>1 t\<^sub>2"
+| tc\<^sub>d_app [simp]: "\<Gamma> \<turnstile>\<^sub>d e\<^sub>1 : Arrow t\<^sub>1 t\<^sub>2 \<Longrightarrow> \<Gamma> \<turnstile>\<^sub>d e\<^sub>2 : t\<^sub>1 \<Longrightarrow> \<Gamma> \<turnstile>\<^sub>d App\<^sub>d e\<^sub>1 e\<^sub>2 : t\<^sub>2"
+
+inductive_cases [elim]: "\<Gamma> \<turnstile>\<^sub>d Var\<^sub>d x : t"
+inductive_cases [elim]: "\<Gamma> \<turnstile>\<^sub>d Const\<^sub>d n : t"
+inductive_cases [elim]: "\<Gamma> \<turnstile>\<^sub>d Lam\<^sub>d t' e : t"
+inductive_cases [elim]: "\<Gamma> \<turnstile>\<^sub>d App\<^sub>d e\<^sub>1 e\<^sub>2 : t"
+
+lemma tc_postpend [simp]: "\<Gamma> \<turnstile>\<^sub>d e : t \<Longrightarrow> (\<Gamma> @ \<Gamma>') \<turnstile>\<^sub>d e : t"
+  by (induction \<Gamma> e t rule: typing\<^sub>d.induct) simp_all
+
+text \<open>We have the same set of values as in our source language:\<close>
+
+primrec value\<^sub>d :: "expr\<^sub>d \<Rightarrow> bool" where
+  "value\<^sub>d (Var\<^sub>d x) = False"
+| "value\<^sub>d (Const\<^sub>d n) = True" 
+| "value\<^sub>d (Lam\<^sub>d t e) = True" 
+| "value\<^sub>d (App\<^sub>d e\<^sub>1 e\<^sub>2) = False" 
+
+lemma canonical_num\<^sub>d [dest]: "\<Gamma> \<turnstile>\<^sub>d e : Num \<Longrightarrow> value\<^sub>d e \<Longrightarrow> \<exists>k. e = Const\<^sub>d k"
+  by (induction \<Gamma> e Num rule: typing\<^sub>d.induct) simp_all
+
+lemma canonical_arrow\<^sub>d [dest]: "\<Gamma> \<turnstile>\<^sub>d e : Arrow t\<^sub>1 t\<^sub>2 \<Longrightarrow> value\<^sub>d e \<Longrightarrow> 
+    \<exists>e'. e = Lam\<^sub>d t\<^sub>1 e' \<and> insert_at 0 t\<^sub>1 \<Gamma> \<turnstile>\<^sub>d e' : t\<^sub>2"
+  by (induction \<Gamma> e "Arrow t\<^sub>1 t\<^sub>2" rule: typing\<^sub>d.induct) simp_all
+
+text \<open>Substitution is much simpler than in our named source language, but not entirely trivial. We 
+need one helper function, to increment all the variables in an expression that are larger than some
+number.\<close>
+
+primrec incr\<^sub>d :: "nat \<Rightarrow> expr\<^sub>d \<Rightarrow> expr\<^sub>d" where
+  "incr\<^sub>d x (Var\<^sub>d y) = Var\<^sub>d (incr x y)"
+| "incr\<^sub>d x (Const\<^sub>d n) = Const\<^sub>d n"
+| "incr\<^sub>d x (Lam\<^sub>d t e) = Lam\<^sub>d t (incr\<^sub>d (Suc x) e)"
+| "incr\<^sub>d x (App\<^sub>d e\<^sub>1 e\<^sub>2) = App\<^sub>d (incr\<^sub>d x e\<^sub>1) (incr\<^sub>d x e\<^sub>2)"
+
+lemma incr\<^sub>d_swap [simp]: "y \<le> x \<Longrightarrow> incr\<^sub>d y (incr\<^sub>d x e) = incr\<^sub>d (Suc x) (incr\<^sub>d y e)"
+  by (induction e arbitrary: x y) simp_all
+
+lemma tc\<^sub>d_incr [simp]: "\<Gamma> \<turnstile>\<^sub>d e : t \<Longrightarrow> x \<le> length \<Gamma> \<Longrightarrow> insert_at x t' \<Gamma> \<turnstile>\<^sub>d incr\<^sub>d x e : t" 
+proof (induction \<Gamma> e t arbitrary: x rule: typing\<^sub>d.induct)
+  case (tc\<^sub>d_app \<Gamma> e\<^sub>1 t\<^sub>1 t\<^sub>2 e\<^sub>2)
+  hence "insert_at x t' \<Gamma> \<turnstile>\<^sub>d (incr\<^sub>d x e\<^sub>1) : Arrow t\<^sub>1 t\<^sub>2" by simp
+  moreover from tc\<^sub>d_app have "insert_at x t' \<Gamma> \<turnstile>\<^sub>d (incr\<^sub>d x e\<^sub>2) : t\<^sub>1" by simp
+  ultimately show ?case by simp
+qed fastforce+
+
+lemma incr\<^sub>d_above_bounds [simp]: "\<Gamma> \<turnstile>\<^sub>d e : t \<Longrightarrow> x \<ge> length \<Gamma> \<Longrightarrow> incr\<^sub>d x e = e"
+proof (induction \<Gamma> e t arbitrary: x rule: typing\<^sub>d.induct)
+  case (tc\<^sub>d_var \<Gamma> y t)
+  moreover hence "y < length \<Gamma>" by simp
+  ultimately have "y < x" by linarith
+  thus ?case by (simp add: incr_min)
+qed simp_all
+
+text \<open>Now we can define substitution. Unlike in our source language, we have to decrement variables 
+that are larger than the substituted variable, because that variable is now gone. In compensation, 
+substitution under a binder is now much easier: we simply increment the variable being substituted 
+for, and also every variable in \<open>e'\<close>.\<close>
+
+primrec subst\<^sub>d :: "nat \<Rightarrow> expr\<^sub>d \<Rightarrow> expr\<^sub>d \<Rightarrow> expr\<^sub>d" where
+  "subst\<^sub>d x e' (Var\<^sub>d y) = (if x = y then e' else Var\<^sub>d (decr x y))"
+| "subst\<^sub>d x e' (Const\<^sub>d n) = Const\<^sub>d n"
+| "subst\<^sub>d x e' (Lam\<^sub>d t e) = Lam\<^sub>d t (subst\<^sub>d (Suc x) (incr\<^sub>d 0 e') e)"
+| "subst\<^sub>d x e' (App\<^sub>d e\<^sub>1 e\<^sub>2) = App\<^sub>d (subst\<^sub>d x e' e\<^sub>1) (subst\<^sub>d x e' e\<^sub>2)"
+
+lemma incr\<^sub>d_subst_swap [simp]: "y \<le> x \<Longrightarrow> 
+    incr\<^sub>d y (subst\<^sub>d x e' e) = subst\<^sub>d (Suc x) (incr\<^sub>d y e') (incr\<^sub>d y e)"
+  by (induction e arbitrary: x y e') (simp_all add: incr_le incr_suc_dest)
+
+lemma subst\<^sub>d_incr_cancel [simp]: "subst\<^sub>d x e' (incr\<^sub>d x e) = e"
+  by (induction e arbitrary: x e') (simp_all, metis incr_not_eq)
+
+lemma subst\<^sub>d_subst_swap [simp]: "y \<le> x \<Longrightarrow> 
+  subst\<^sub>d x e\<^sub>1 (subst\<^sub>d y e\<^sub>2 e) = subst\<^sub>d y (subst\<^sub>d x e\<^sub>1 e\<^sub>2) (subst\<^sub>d (Suc x) (incr\<^sub>d y e\<^sub>1) e)"
+proof (induction e arbitrary: x y e\<^sub>1 e\<^sub>2)
+  case (Var\<^sub>d z)
+  thus ?case 
+  proof (cases "y = z")
+    case False
+    with Var\<^sub>d show ?thesis 
+    proof (cases "x = decr y z")
+      case True note TXD = True
+      with Var\<^sub>d False show ?thesis
+      proof (cases "y = decr y z")
+        case True
+        with False have "z = Suc y" by simp
+        with TXD show ?thesis by auto
+      qed simp_all
+    qed auto
+  qed simp_all
+qed simp_all
+
+lemma tc\<^sub>d_subst [simp]: "insert_at x t' \<Gamma> \<turnstile>\<^sub>d e : t \<Longrightarrow> x \<le> length \<Gamma> \<Longrightarrow> \<Gamma> \<turnstile>\<^sub>d e' : t' \<Longrightarrow> 
+  \<Gamma> \<turnstile>\<^sub>d subst\<^sub>d x e' e : t"
+proof (induction "insert_at x t' \<Gamma>" e t arbitrary: \<Gamma> x e' rule: typing\<^sub>d.induct)
+  case (tc\<^sub>d_var y t)
+  moreover have "x \<le> length \<Gamma> \<Longrightarrow> x \<noteq> y \<Longrightarrow> lookup \<Gamma> (decr x y) = lookup (insert_at x t' \<Gamma>) y" 
+    by simp
+  ultimately show ?case by fastforce
+qed fastforce+ 
+
+lemma subst\<^sub>d_above_bounds [simp]: "\<Gamma> \<turnstile>\<^sub>d e : t \<Longrightarrow> x \<ge> length \<Gamma> \<Longrightarrow> subst\<^sub>d x e' e = e"
+proof (induction \<Gamma> e t arbitrary: x e' rule: typing\<^sub>d.induct)
+  case (tc\<^sub>d_var \<Gamma> y t)
+  hence "y < length \<Gamma>" by simp
+  with tc\<^sub>d_var have "y < x" by linarith
+  with tc\<^sub>d_var show ?case by auto
+qed simp_all
+
+lemma subst\<^sub>d_to_var [dest]: "subst\<^sub>d 0 e' e = Var\<^sub>d x \<Longrightarrow> value\<^sub>d e' \<Longrightarrow> e = Var\<^sub>d (Suc x)"
+proof (induction e)
+  case (Var\<^sub>d y)
+  thus ?case by (induction y) simp_all
+qed simp_all
+
+lemma value\<^sub>d_subst [dest]: "value\<^sub>d (subst\<^sub>d 0 e' e) \<Longrightarrow> value\<^sub>d e' \<Longrightarrow> value\<^sub>d e \<or> e = Var\<^sub>d 0"
+  by (induction e) (simp_all split: if_splits)
+
+text \<open>We can now define evaluation. Unlike our source language, but in keeping with future stages, 
+we use a small-step evaluation relation. (We will define big-step evaluation for this stage 
+subsequently.) This will allow us, for the first time, to prove the full safety property.\<close>
+
+inductive eval\<^sub>d :: "expr\<^sub>d \<Rightarrow> expr\<^sub>d \<Rightarrow> bool" (infix "\<leadsto>\<^sub>d" 50) where
+  ev\<^sub>d_app1 [simp]: "e\<^sub>1 \<leadsto>\<^sub>d e\<^sub>1' \<Longrightarrow> App\<^sub>d e\<^sub>1 e\<^sub>2 \<leadsto>\<^sub>d App\<^sub>d e\<^sub>1' e\<^sub>2"
+| ev\<^sub>d_app2 [simp]: "value\<^sub>d e\<^sub>1 \<Longrightarrow> e\<^sub>2 \<leadsto>\<^sub>d e\<^sub>2' \<Longrightarrow> App\<^sub>d e\<^sub>1 e\<^sub>2 \<leadsto>\<^sub>d App\<^sub>d e\<^sub>1 e\<^sub>2'"
+| ev\<^sub>d_app3 [simp]: "value\<^sub>d e\<^sub>2 \<Longrightarrow> App\<^sub>d (Lam\<^sub>d t e\<^sub>1) e\<^sub>2 \<leadsto>\<^sub>d subst\<^sub>d 0 e\<^sub>2 e\<^sub>1"
+
+lemma val_no_eval\<^sub>d: "e \<leadsto>\<^sub>d e' \<Longrightarrow> value\<^sub>d e \<Longrightarrow> False"
+  by (induction e e' rule: eval\<^sub>d.induct) simp_all
+
+text \<open>Our metatheoretic properties, progress, preservation, and determinism, now all follow 
+straightforwardly.\<close>
+
+theorem progress\<^sub>d: "[] \<turnstile>\<^sub>d e : t \<Longrightarrow> value\<^sub>d e \<or> (\<exists>e'. e \<leadsto>\<^sub>d e')"
+proof (induction "[] :: ty list" e t rule: typing\<^sub>d.induct)
+  case (tc\<^sub>d_app e\<^sub>1 t\<^sub>1 t\<^sub>2 e\<^sub>2)
+  thus ?case 
+  proof (cases "value\<^sub>d e\<^sub>1")
+    case True note T = True
+    thus ?thesis 
+    proof (cases "value\<^sub>d e\<^sub>2")
+      case True
+      with tc\<^sub>d_app T show ?thesis by (metis canonical_arrow\<^sub>d ev\<^sub>d_app3)
+    next
+      case False
+      with tc\<^sub>d_app T show ?thesis by (metis ev\<^sub>d_app2)
+    qed
+  next
+    case False
+    with tc\<^sub>d_app show ?thesis by (metis ev\<^sub>d_app1)
+  qed
+qed simp_all
+
+theorem preservationd [simp]: "e \<leadsto>\<^sub>d e' \<Longrightarrow> \<Gamma> \<turnstile>\<^sub>d e : t \<Longrightarrow> \<Gamma> \<turnstile>\<^sub>d e' : t"
+  by (induction e e' arbitrary: t rule: eval\<^sub>d.induct) fastforce+
+
+theorem determinism\<^sub>d: "e \<leadsto>\<^sub>d e' \<Longrightarrow> e \<leadsto>\<^sub>d e'' \<Longrightarrow> e' = e''"
+proof (induction e e' arbitrary: e'' rule: eval\<^sub>d.induct)
+case (ev\<^sub>d_app1 e\<^sub>1 e\<^sub>1' e\<^sub>2)
+  from ev\<^sub>d_app1(3, 1, 2) show ?case 
+    using val_no_eval\<^sub>d value\<^sub>d.simps(3) by (induction rule: eval\<^sub>d.cases) blast+
+next
+  case (ev\<^sub>d_app2 e\<^sub>1 e\<^sub>2 e\<^sub>2')
+  from ev\<^sub>d_app2(4, 1, 2, 3) show ?case 
+     using val_no_eval\<^sub>d by (induction rule: eval\<^sub>d.cases) blast+
+next
+  case (ev\<^sub>d_app3 e\<^sub>2 t e\<^sub>1)
+  from ev\<^sub>d_app3(2, 1) show ?case 
+    using val_no_eval\<^sub>d value\<^sub>d.simps(3) by (induction rule: eval\<^sub>d.cases) blast+
+qed
+
+end
